\documentclass[12pt]{article}

\usepackage[utf8]{inputenc}
\usepackage[T2A]{fontenc}

\usepackage{parskip}
\usepackage{amsmath}
\usepackage{amssymb}

\begin{document}

\center{Reduce lambda term to the normal form:}
\[ ((\lambda a.(\lambda b.b \ b) \ (\lambda b.b \ b)) \ b) \ ((\lambda c.(c \ b)) \ (\lambda a.a)) \rightarrow_\beta \]
\[ \rightarrow_\beta ((\lambda b.b \ b) \ (\lambda b.b \ b)) \ ((\lambda c.(c \ b)) \ (\lambda a.a)) \rightarrow_\beta \]
\[ \rightarrow_\beta ((\lambda b.b \ b) \ (\lambda b.b \ b)) \ ((\lambda a.a) \ b) \rightarrow_\beta \]
\[ \rightarrow_\beta ((\lambda b.b \ b) \ (\lambda b.b \ b)) \ b \equiv \]
\[ \equiv \Omega \ b \]

\end{document}
